\documentclass{article}
\usepackage{epsfig}
\pagestyle{empty}
\begin{document}
$ \ell^p $
\pagebreak

$ \ell^p\infty $
\pagebreak

$ A x = b $
\pagebreak

$ b = A^{-1} b $
\pagebreak

$ {L^{*}}^{-1} D^{-1} L^{-1} b $
\pagebreak

$ {L^{*}}^{-1} L^{-1} b $
\pagebreak

$ v $
\pagebreak

$ w $
\pagebreak

$ p $
\pagebreak

\[ \Vert v - w \Vert \leqslant p\,\min(\Vert v\Vert, \Vert w\Vert). \]
\pagebreak

$ x $
\pagebreak

\[ \Vert v \Vert \leqslant p\,\vert x\vert. \]
\pagebreak

\[ \Vert v \Vert \leqslant p\,\Vert w\Vert. \]
\pagebreak

$ n \cdot x + d = 0 $
\pagebreak

$ n $
\pagebreak

$ d $
\pagebreak

$ c_0*x_0 + ... + c_{d-1}*x_{d-1} + c_d = 0 $
\pagebreak

$ \mathbf{o} $
\pagebreak

$ \mathbf{d} $
\pagebreak

$ l(t) = \mathbf{o} + t \mathbf{d} $
\pagebreak

$ l \in \mathbf{R} $
\pagebreak

$ w+xi+yj+zk $
\pagebreak

$(x,y,z)$
\pagebreak

$y$
\pagebreak

$x$
\pagebreak

$z$
\pagebreak

\[ y=ax+bz+c \]
\pagebreak

$a,b,c$
\pagebreak

$y=ax+bz+c$
\pagebreak

$( 0.495 , -1.927 , -2.906 )$
\pagebreak

$a=0.495, b = -1.927, c = -2.906$
\pagebreak

\[ax+bz+c = 0.495 * 3.02 + (-1.927) * (-4.32) + (-2.906) = 6.91.\]
\pagebreak

$y=6.89$
\pagebreak

$6.91$
\pagebreak

$6.89$
\pagebreak

$n=Size$
\pagebreak

$r_i=result[i]$
\pagebreak

$f=funcOfOthers$
\pagebreak

$x_0,\ldots,x_{n-1}$
\pagebreak

\[ x_f = r_0 x_0 + \cdots + r_{f-1}x_{f-1} + r_{f+1}x_{f+1} + \cdots + r_{n-1}x_{n-1} + r_n. \]
\pagebreak

\[ r_0 x_0 + \cdots + r_{n-1}x_{n-1} + r_n = 0, \]
\pagebreak

$r_i=retCoefficients[i]$
\pagebreak

$n+1$
\pagebreak

$ \left[ \begin{array}{cccccc} u+iv & & & & & \\ & u-iv & & & & \\ & & a+ib & & & \\ & & & a-ib & & \\ & & & & x & \\ & & & & & y \\ \end{array} \right] $
\pagebreak

$ D =\left[ \begin{array}{cccccc} u & v & & & & \\ -v & u & & & & \\ & & a & b & & \\ & & -b & a & & \\ & & & & x & \\ & & & & & y \\ \end{array} \right] $
\pagebreak

$ A $
\pagebreak

$ A = Q H Q^* $
\pagebreak

$ Q $
\pagebreak

$ H $
\pagebreak

$ Ax = lambda B x $
\pagebreak

$ B $
\pagebreak

$ A = Q T Q^* $
\pagebreak

$ T $
\pagebreak

$\cdot value2 - value1 <= abs(intervalSize * 10e^{-6})$
\pagebreak

$y = f([x1,x2])$
\pagebreak

$[y1,y2] = f(x)$
\pagebreak

$stepSize = (intervalSize - intervalSize * 10e^{-6}) / numSteps$
\pagebreak

$\left\{ 1,2,5\right\} \cdot 10^{n}$
\pagebreak

$\left\{ 1,2,3,5\right\} \cdot 10^{n}$
\pagebreak

\end{document}
